Make some things instances

src/Specific/GF25519Bounded.v
@@ -281,12 +281,16 @@ Proof.
   { cbv [decode encode div]; intros; rewrite !proj1_fe25519_exist_fe25519; apply encode_rep. }
 Qed.
 
-Definition field25519 : @field fe25519 eq zero one opp add sub mul inv div := proj1 field25519_and_homomorphisms.
+Global Instance field25519 : @field fe25519 eq zero one opp add sub mul inv div := proj1 field25519_and_homomorphisms.
 
 Local Opaque proj1_fe25519 exist_fe25519 proj1_fe25519W exist_fe25519W.
-Lemma homomorphism_F25519 :
+Global Instance homomorphism_F25519 :
   @Ring.is_homomorphism
     (F modulus) Logic.eq F.one F.add F.mul
     fe25519 eq one add mul encode.
+Proof. apply field25519_and_homomorphisms. Qed.
+
+Global Instance homomorphism_F25519_decode
+  : @Ring.is_homomorphism fe25519 eq one add mul (F _) (@Logic.eq _) 1%F F.add F.mul decode.
 Proof. apply field25519_and_homomorphisms. Qed.
 (** TODO: pack, unpack, ge_modulus *)
